Buffers: new equations for singleton buffers from array cells

ulib/FStar.Pointer.Base.fst
@@ -124,9 +124,14 @@ let g_is_null_intro
 
 (** Buffers *)
 
+let not_an_array_cell (#t: typ) (p: pointer t) : GTot bool =
+  match Pointer?.p p with
+  | PathStep _ _ _ (StepCell _ _ _) -> false
+  | _ -> true
+
 noeq type buffer_root (t: typ) =
 | BufferRootSingleton:
-  (p: pointer t) ->
+  (p: pointer t { not_an_array_cell p } ) ->
   buffer_root t
 | BufferRootArray:
   (#max_length: array_length_t) ->
@@ -2551,19 +2556,21 @@ let is_active_union_field_includes_readable
 
 (** Operations on buffers *)
 
-let gsingleton_buffer_of_pointer
+let _singleton_buffer_of_pointer
   (#t: typ)
   (p: pointer t)
-: GTot (buffer t)
-= Buffer (BufferRootSingleton p) 0ul 1ul
+: Tot (buffer t)
+= let Pointer from contents pth = p in
+  match pth with
+  | PathStep _ _ pth' (StepCell ln ty i) ->
+    (* reconstruct the buffer to the enclosing array *)
+    Buffer (BufferRootArray #ty #ln (Pointer from contents pth')) i 1ul 
+  | _ ->
+    Buffer (BufferRootSingleton p) 0ul 1ul
 
-let singleton_buffer_of_pointer
-  (#t: typ)
-  (p: pointer t)
-: HST.Stack (buffer t)
-  (requires (fun h -> live h p))
-  (ensures (fun h b h' -> h' == h /\ b == gsingleton_buffer_of_pointer p))
-= Buffer (BufferRootSingleton p) 0ul 1ul
+let gsingleton_buffer_of_pointer #t p = _singleton_buffer_of_pointer p
+
+let singleton_buffer_of_pointer #t p = _singleton_buffer_of_pointer p
 
 let gbuffer_of_array_pointer
   (#t: typ)
@@ -2753,11 +2760,26 @@ let buffer_length_buffer_as_seq
   (b: buffer t)
 = ()
 
-let buffer_as_seq_gsingleton_buffer_of_pointer
-  (#t: typ)
-  (h: HS.mem)
-  (p: pointer t)
-= Seq.slice_length (Seq.create 1 (gread h p))
+let buffer_as_seq_gsingleton_buffer_of_pointer #t h p =
+  let Pointer from contents pth = p in
+  match pth with
+  | PathStep through to pth' (StepCell ln ty i) ->
+    assert (through == TArray ln ty);
+    assert (to == ty);
+    assert (t == ty);
+    let p' : pointer (TArray ln ty) = Pointer from contents pth' in
+    let s : array ln (type_of_typ t) = gread h p' in
+    let s1 = Seq.slice s (UInt32.v i) (UInt32.v i + 1) in
+    let v = gread h p in
+    assert (v == Seq.index s (UInt32.v i));
+    let s2 = Seq.create 1 v in
+    assert (Seq.length s1 == 1);
+    assert (Seq.length s2 == 1);
+    assert (Seq.index s1 0 == v);
+    assert (Seq.index s2 0 == v);
+    assert (Seq.equal s1 s2)
+  | _ ->
+    Seq.slice_length (Seq.create 1 (gread h p))
 
 let buffer_as_seq_gbuffer_of_array_pointer
   (#length: array_length_t)
@@ -2842,6 +2864,10 @@ let index_buffer_as_seq
   (b: buffer t)
   i
 = ()
+
+let gsingleton_buffer_of_pointer_gcell #t #len p i = ()
+
+let gsingleton_buffer_of_pointer_gpointer_of_buffer_cell #t b i = ()
 
 (* The readable permission lifted to buffers. *)
 
@@ -4081,17 +4107,8 @@ let live_unused_in_disjoint_strong
   (ensures (frameOf p1 <> frameOf p2 \/ as_addr p1 <> as_addr p2))
 = ()
 
-let live_unused_in_disjoint
-  (#value1: typ)
-  (#value2: typ)
-  (h: HS.mem)
-  (p1: pointer value1)
-  (p2: pointer value2)
-: Lemma
-  (requires (live h p1 /\ unused_in p2 h))
-  (ensures (disjoint p1 p2))
-  [SMTPatT (disjoint p1 p2); SMTPatT (live h p1)]
-= live_unused_in_disjoint_strong h p1 p2;
+let live_unused_in_disjoint #value1 #value2 h p1 p2 =
+  live_unused_in_disjoint_strong h p1 p2;
   disjoint_root p1 p2
 
 let loc_disjoint_gsub_buffer #t b i1 len1 i2 len2 = ()
